src/Minimal.Hardware.fst
@@ -14,7 +14,41 @@ module HST = FStar.HyperStack.ST
 module B = LowStar.Buffer
 
 let uds_len = 0x20ul
+let header_len = 0x20ul
+let entry_t = unit -> HST.St unit
+let entry = fun () -> ()
 
+noeq
+type header_t = {
+     (* actual entries in headers*)
+     binary_size   : binary_size_t;
+     binary_hash   : digest_t;
+     header_sig    : signature_t;
+     (* extra entries for convenience *)
+     binary        : B.lbuffer uint8 (v binary_size);
+     header_raw    : header_raw_t;
+     header_pubkey : publickey_t;
+     entry         : entry_t;
+     header_inv    : u:unit{
+       B.(all_disjoint [ loc_buffer binary_hash
+                       ; loc_buffer header_sig
+                       ; loc_buffer binary
+                       ; loc_buffer header_raw
+                       ; loc_buffer header_pubkey
+       ])
+     }
+}
+
+let get_binary_size header = header.binary_size
+let get_binary_hash header = header.binary_hash
+let get_header_sig  header = header.header_sig
+let get_binary      header = header.binary
+let get_header_raw  header = header.header_raw
+let get_header_pubkey header = header.header_pubkey
+let get_entry       header = header.entry
+
+/// <><><><><><><><><><><><> Monotonic Predicates <><><><><><><><><><><><>
+/// 
 noextract
 type t =
   | Uninitialized
@@ -51,39 +85,83 @@ let uds_is_disabled_predicate : HST.mem_predicate =
 
 let uds_is_disabled = HST.token_p local_state_ref uds_is_disabled_predicate
 
+/// <><><><><><><><><><><><><><><><> State <><><><><><><><><><><><><><><><>
+
 noeq
 type state = {
   uds     : B.buffer uint8;
   cdi     : B.buffer uint8;
+  header  : header_t;
   uds_val : s:G.erased (Seq.seq uint8){
     B.length uds == v uds_len /\
     B.length cdi == v cdi_len /\
     Seq.length (G.reveal s) == v uds_len /\
     B.freeable uds /\
     B.freeable cdi /\
-    B.all_disjoint [ B.loc_buffer uds
+    B.all_disjoint ([B.loc_buffer uds
                    ; B.loc_buffer cdi
-                   ; B.loc_mreference local_state_ref]
+                   ; B.loc_mreference local_state_ref] @
+                   (get_header_loc_l header))
   }
 }
 
 let get_uds st = st.uds
 let get_cdi st = st.cdi
+let get_header st = st.header
 let get_uds_value st = G.reveal st.uds_val
 
-let initialize riot_binary =
+let load_header
+  (_: unit)
+: HST.ST (header: header_t)
+  (requires fun h -> True)
+  (ensures fun h0 header h1 -> True)
+=
+  let binary_size:binary_size_t   = 100ul in
+  let binary_hash   = B.malloc HS.root (u8 0x00) digest_len in
+  let header_sig    = B.malloc HS.root (u8 0x00) 64ul in
+  let binary        = B.malloc HS.root (u8 0x00) binary_size in
+  let header_raw    = B.malloc HS.root (u8 0x00) header_len in
+  let header_pubkey = B.malloc HS.root (u8 0x00) 32ul in
+  { binary_size = binary_size
+  ; binary_hash = binary_hash
+  ; header_sig  = header_sig
+  ; binary      = binary
+  ; header_raw  = header_raw
+  ; header_pubkey = header_pubkey
+  ; entry       = entry
+  ; header_inv  = () }
+
+#reset-options "--z3rlimit 50"
+#push-options "--query_stats"
+let initialize () =
   HST.recall local_state_ref;
-  local_state_ref `HST.op_Colon_Equals` (G.hide Enabled);
+  HST.(local_state_ref := Enabled);
   HST.witness_p local_state_ref uds_is_initialized_predicate;
 
   let uds = B.malloc HS.root (u8 0x00) uds_len in
   let cdi = B.malloc HS.root (u8 0x00) uds_len in
+  let binary_size   = 100ul in
+  let binary_hash   = B.malloc HS.root (u8 0x00) digest_len in
+  let header_sig    = B.malloc HS.root (u8 0x00) 64ul in
+  let binary        = B.malloc HS.root (u8 0x00) binary_size in
+  let header_raw    = B.malloc HS.root (u8 0x00) header_len in
+  let header_pubkey = B.malloc HS.root (u8 0x00) 32ul in
 
   let uds_seq =
     let h = HST.get () in
     G.hide (B.as_seq h uds) in
 
-  { uds = uds; cdi = cdi; uds_val = uds_seq }
+  { uds = uds
+  ; cdi = cdi
+  ; header  = { binary_size = binary_size
+              ; binary_hash = binary_hash
+              ; header_sig  = header_sig
+              ; binary      = binary
+              ; header_raw  = header_raw
+              ; header_pubkey = header_pubkey
+              ; entry       = entry
+              ; header_inv  = () }
+  ; uds_val = uds_seq }
 
 let unset_uds st =
   let uds = get_uds st in
@@ -93,7 +171,7 @@ let unset_uds st =
 
 let disable_uds st =
   HST.recall_p local_state_ref uds_is_initialized_predicate;
-  local_state_ref `HST.op_Colon_Equals` Disabled;
+  HST.(local_state_ref := Disabled);
   HST.witness_p local_state_ref uds_is_disabled_predicate;
 
   B.free st.uds
