src/Minimal.Loader.fsti
@@ -23,66 +23,6 @@ module HS  = FStar.HyperStack
 module HST = FStar.HyperStack.ST
 module CString = C.String
 
-let binary_len_t = a:size_t{0 < v a /\ v a <= max_input_length alg}
-
-val header_len: binary_len_t
-
-let version_number_t = pub_uint32
-let signature_t = B.lbuffer uint8 64
-let publickey_t = B.lbuffer uint8 32
-let secretkey_t = B.lbuffer uint8 32
-let msg_len_t = a:size_t{v a + 64 <= max_size_t}
-
-let header_raw_t = B.lbuffer uint8 (v header_len)
-
-(* ZT: plan to hide this definition in the next revision *)
-noeq
-type header_t = {
-     (* actual entries in headers*)
-     version        : version_number_t;
-     binary_size    : riot_size_t;
-     binary_hash    : digest_t;
-     header_sig     : signature_t;
-     (* extra entries for convenience *)
-     binary         : B.lbuffer uint8 (v binary_size);
-     header_raw     : header_raw_t;
-     header_pubkey  : publickey_t
-}
-
-unfold noextract
-let contains_header (h:HS.mem) (header: header_t) =
-  B.live h header.binary_hash /\
-  B.live h header.header_sig /\
-  B.live h header.header_raw /\
-  B.live h header.header_pubkey
-
-unfold noextract
-let get_header_loc_l header = [B.loc_buffer header.binary_hash
-                               ;B.loc_buffer header.header_sig
-                               ;B.loc_buffer header.header_raw
-                               ;B.loc_buffer header.header_pubkey]
-
-(* ZT: plan to revise this definition *)
-val entry_t: Type0
-val entry: entry_t
-
-noeq
-type layer_t = {
-  size   : binary_len_t;
-  binary : B.lbuffer uint8 (v size);
-  entry  : entry_t
-}
-
-(* ZT: only thing in C *)
-val load_header
-  (_: unit)
-: HST.ST (header: header_t)
-  (requires fun h -> True)
-  (ensures fun h0 header h1 -> B.(
-    all_disjoint (get_header_loc_l header) /\
-    modifies loc_none h0 h1 /\
-    h1 `contains_header` header))
-
 #reset-options "--z3rlimit 30"
 let verify_header
   (header: header_t)
@@ -91,31 +31,12 @@ let verify_header
     h `contains_header` header /\
     B.all_disjoint (get_header_loc_l header))
   (ensures  fun h0 b h1 ->
-    let rhDigest_seq = Spec.Agile.Hash.hash alg (B.as_seq h0 header.header_raw) in
-    Spec.Ed25519.verify (B.as_seq h0 header.header_pubkey) rhDigest_seq (B.as_seq h0 header.header_sig) == b)
+    let rhDigest_seq = Spec.Agile.Hash.hash alg (B.as_seq h0 (get_header_raw header)) in
+    Spec.Ed25519.verify (B.as_seq h0 (get_header_pubkey header)) rhDigest_seq (B.as_seq h0 (get_header_sig header)) == b)
 =
   HST.push_frame ();
   let rhDigest = B.alloca (u8 0x00) digest_len in
-  dice_hash alg header.header_raw header_len rhDigest;
-  let b = Ed25519.verify header.header_pubkey digest_len rhDigest header.header_sig in
+  dice_hash alg (get_header_raw header) header_len rhDigest;
+  let b = Ed25519.verify (get_header_pubkey header) digest_len rhDigest (get_header_sig header) in
   HST.pop_frame ();
   b
-
-let load_layer
-  (_: unit)
-: HST.ST (layer: layer_t)
-  (requires fun h -> True)
-  (ensures  fun h0 layer h1 ->
-    B.live h1 layer.binary)
-=
-  let header = load_header () in
-  let layer: layer_t = {
-    size   = header.binary_size;
-    binary = B.malloc HS.root (u8 0x00) header.binary_size;
-    entry  = entry } in
-  let verify_result = verify_header header in
-  (**)assume (verify_result == true);
-  (**)assert (verify_result == true);
-  (* ZT: no dynamic failures in F* *)
-  if (verify_result) then () else (C.exit (-1l));
-  layer
